dafny/play.dfy
@@ -1,8 +1,0 @@
-   method Main() {
-       var l := [1,2,3];
-       var j := [1,8];
-       print(j[..1]);
-       assert j[..1] == [j[0]];
-      //  print(l[..|l|]);
-      //  print(forall v :: 0 <= v < |j| ==> j[v] in l);
-    }
